Fix dev until last Lemma in CombineEnv.v/transval.v

TransVal/Compute.v
@@ -1,5 +1,5 @@
 Require Import IL StateType.
-Require Import smt noGoto.
+Require Import smt.
 
 Set Implicit Arguments.
 
@@ -7,27 +7,27 @@ Inductive Terminates :F.state -> F.state -> Prop :=
 |TerminatesReturn L E e v:
    exp_eval E e = ⎣v⎦
    -> Terminates (L, E, stmtReturn e)   (L  , E , stmtReturn e)
-|TerminatesGoto L E f x vl:
+|TerminatesApp L E f x vl:
    omap (exp_eval E) x = ⎣vl⎦
-   -> Terminates (L, E, stmtGoto f x) (L, E, stmtGoto f x)
+   -> Terminates (L, E, stmtApp f x) (L, E, stmtApp f x)
 |TerminatesStep L E s L'  E' s'  L'' E'' s''  a:
    F.step (L, E, s) a (L', E', s')
    -> Terminates (L', E', s') (L'', E'', s'')
-   ->  (forall f xl, s <> stmtGoto f xl)
+   ->  (forall f xl, s <> stmtApp f xl)
    -> Terminates (L,E,s) (L'', E'', s'') .
 
 Inductive Crash : F.state -> F.state -> Prop :=
-|CrashGoto L E f Y:
+|CrashApp L E f Y:
 omap (exp_eval E) Y = None
--> Crash (L, E, stmtGoto f Y) (L, E, stmtGoto f Y)
+-> Crash (L, E, stmtApp f Y) (L, E, stmtApp f Y)
 |CrashBase L E s :
-( forall f el, s <> stmtGoto f el)
+( forall f el, s <> stmtApp f el)
 ->  normal2 F.step (L, E, s)
 -> state_result (L,E,s) = None
 -> Crash (L, E,s) (L,E,s)
 |CrashStep L E s sigma' sigma'' a:
    F.step (L, E, s) a sigma'
-   ->  (forall f xl, s <> stmtGoto f xl)
+   ->  (forall f xl, s <> stmtApp f xl)
    -> Crash sigma' sigma''
    -> Crash (L,E,s) sigma''.
 
