TransVal/CombineEnv.v
@@ -1,7 +1,7 @@
 Require Import List Arith.
-Require Import IL Annotation AutoIndTac Bisim Exp MoreExp Coherence Fresh Util.
+Require Import IL Annotation AutoIndTac Exp MoreExp RenamedApart Fresh Util.
 Require Import SetOperations Sim Var.
-Require Import bitvec smt nofun noGoto freeVars.
+Require Import bitvec smt nofun freeVars.
 Require Import Compute Guards ILFtoSMT tvalTactics TUtil GuardProps ComputeProps.
 
 (** Definitons **)
@@ -14,7 +14,7 @@ Lemma combineenv_agree D E E':
   agree_on eq D (combineEnv D E E') E.
 
 Proof.
-  hnf; intros. unfold combineEnv. destruct if; eauto; isabsurd.
+  hnf; intros. unfold combineEnv. cases; eauto; isabsurd.
 Qed.
 
 Lemma exp_combineenv_eql:
@@ -73,10 +73,10 @@ agree_on eq (Exp.freeVars e ∩ D) Es Et
 Proof.
  intros; split; intros.
  - eapply (exp_eval_agree (E:=(combineEnv D Es Et))); eauto.
-   hnf. cset_tac. unfold combineEnv. destruct if; eauto.
+   hnf. cset_tac. unfold combineEnv. cases; eauto.
    eapply H. cset_tac; intuition.
  - eapply (exp_eval_agree (E:= Et)); eauto.
-   hnf; cset_tac. unfold combineEnv; destruct if; eauto.
+   hnf; cset_tac. unfold combineEnv; cases; eauto.
    symmetry. eapply H; cset_tac; intuition.
 Qed.
 
@@ -89,10 +89,10 @@ agree_on eq (Exp.freeVars e ∩ D) Es Et
 Proof.
  intros; split; intros.
  - eapply (exp_eval_agree (E:=(to_partial (to_total (combineEnv D Es Et))))); eauto.
-   hnf. cset_tac. unfold combineEnv, to_partial, to_total. destruct if; eauto.
+   hnf. cset_tac. unfold combineEnv, to_partial, to_total. cases; eauto.
    rewrite H. reflexivity. cset_tac; intuition.
  - eapply (exp_eval_agree (E:= to_partial (to_total Et))); eauto.
-   hnf; cset_tac. unfold combineEnv, to_partial, to_total; destruct if; eauto.
+   hnf; cset_tac. unfold combineEnv, to_partial, to_total; cases; eauto.
    rewrite H. reflexivity.
    cset_tac; intuition.
 Qed.
@@ -110,22 +110,22 @@ Proof.
       pose proof (exp_combineenv_eqr a D Es Et (exp_eval (combineEnv D Es Et) a)).
       destruct H0.
       * hnf; intros; cset_tac. eapply H. split; eauto.
-        unfold list_union; simpl. eapply list_union_start_swap; cset_tac; eauto.
+        eapply list_union_start_swap; cset_tac; eauto.
       * rewrite H0; eauto. f_equal.
         rewrite (IHel D Es Et (omap (exp_eval (combineEnv D Es Et)) el)); eauto.
         hnf. intros. cset_tac. eapply H. split; eauto.
-        unfold list_union. simpl. eapply list_union_start_swap. cset_tac; eauto.
+        eapply list_union_start_swap. cset_tac; eauto.
   - general induction el.
     + reflexivity.
     + simpl in *; hnf in H.
       pose proof (exp_combineenv_eqr a D Es Et (exp_eval Et a)).
       destruct H0.
       * hnf; intros; cset_tac. eapply H. split; eauto.
-        unfold list_union; simpl. eapply list_union_start_swap; cset_tac; eauto.
+        eapply list_union_start_swap; cset_tac; eauto.
       * rewrite H1; eauto. f_equal.
         symmetry. rewrite (IHel D Es Et (omap (exp_eval  Et) el)); eauto.
         hnf. intros. cset_tac. eapply H. split; eauto.
-        unfold list_union. simpl. eapply list_union_start_swap. cset_tac; eauto.
+        eapply list_union_start_swap. cset_tac; eauto.
 Qed.
 
 Lemma explist_combineenv_eqr':
@@ -142,24 +142,24 @@ Proof.
       pose proof (exp_combineenv_eqr' a D Es Et (exp_eval (to_partial (to_total (combineEnv D Es Et))) a)).
       destruct H0.
       * hnf; intros; cset_tac. eapply H; split; eauto.
-        unfold list_union; simpl; eapply list_union_start_swap; cset_tac; eauto.
+        eapply list_union_start_swap; cset_tac; eauto.
       * rewrite H0; eauto. f_equal.
         symmetry. simpl.
         rewrite (IHel D Es Et (omap (exp_eval (to_partial (to_total (combineEnv D Es Et)))) el)); eauto.
         hnf; intros; cset_tac. eapply H; split; eauto.
-        unfold list_union; simpl; eapply list_union_start_swap. cset_tac; eauto.
+        eapply list_union_start_swap. cset_tac; eauto.
   - general induction el.
     + reflexivity.
     + simpl in *; hnf in H.
       pose proof (exp_combineenv_eqr' a D Es Et (exp_eval (to_partial (to_total Et)) a)).
       destruct H0.
       * hnf; intros; cset_tac. eapply H; split; eauto.
-        unfold list_union; simpl; eapply list_union_start_swap; cset_tac; eauto.
+        eapply list_union_start_swap; cset_tac; eauto.
       * rewrite H1; eauto. f_equal.
         symmetry. simpl.
         rewrite (IHel D Es Et (omap (exp_eval (to_partial (to_total Et))) el)); eauto.
         hnf; intros; cset_tac. eapply H; split; eauto.
-        unfold list_union; simpl; eapply list_union_start_swap. cset_tac; eauto.
+        eapply list_union_start_swap. cset_tac; eauto.
 Qed.
 
 Lemma combineenv_eqr:
@@ -183,8 +183,7 @@ Proof.
   - case_eq (exp_eval (to_partial (to_total (combineEnv D Es Et))) e); intros.
     + pose proof (exp_combineenv_eqr' e D Es Et (Some v)).
       assert (agree_on eq (Exp.freeVars e ∩ D) Es Et).
-      * hnf; intros. hnf in H. simpl in H. cset_tac. eapply H.
-        split; eauto.
+      * hnf; intros. hnf in H. simpl in H. cset_tac.
       * destruct H1; eauto.
         specialize (H1 H0).
         unfold smt_eval; rewrite H1.
@@ -197,8 +196,7 @@ Proof.
           - setSubst2 H. }
      + pose proof (exp_combineenv_eqr' e D Es Et None).
        assert (agree_on eq (Exp.freeVars e ∩ D) Es Et).
-       * hnf; intros. hnf in H. simpl in H. cset_tac. eapply H.
-         split; eauto.
+       * hnf; intros. hnf in H. simpl in H. cset_tac.
        * destruct H1; eauto.  specialize (H1 H0).
          unfold smt_eval; rewrite H0, H1.
          case_eq (val2bool undef_substitute); intros.
@@ -216,13 +214,11 @@ Proof.
     case_eq (exp_eval (to_partial (to_total (combineEnv D Es Et))) e0); intros.
     + pose proof (exp_combineenv_eqr' e D Es Et (Some v)).
        assert (agree_on eq (Exp.freeVars e ∩ D) Es Et).
-       * hnf; intros. hnf in H. simpl in H. cset_tac. eapply H.
-         split; eauto.
+       * hnf; intros. hnf in H. simpl in H. cset_tac.
        * destruct H2; eauto. specialize (H2 H0).
          pose proof (exp_combineenv_eqr' e0 D Es Et (Some v0)).
          assert (agree_on eq (Exp.freeVars e0 ∩ D) Es Et).
-       { hnf; intros. hnf in H. simpl in H. cset_tac. eapply H.
-         split; eauto. }
+       { hnf; intros. hnf in H. simpl in H. cset_tac. }
        { destruct H5; eauto. specialize (H5 H1).
          unfold smt_eval.
          rewrite H2, H5, H4, H7; eauto; intuition.
@@ -269,11 +265,9 @@ Proof.
          pose proof (exp_combineenv_eqr' a D Es Et
                                          (exp_eval (to_partial (to_total (combineEnv D Es Et))) a)).
          destruct H0.
-         { setSubst2 H. unfold list_union; simpl.
-           eapply list_union_start_swap; cset_tac; eauto. }
+         { setSubst2 H. eapply list_union_start_swap; cset_tac; eauto. }
          { destruct H1.
-           - setSubst2 H. unfold list_union; simpl.
-           eapply list_union_start_swap; cset_tac; eauto.
+           - setSubst2 H. eapply list_union_start_swap; cset_tac; eauto.
            - clear H3. clear H0.
              unfold smt_eval at 1. rewrite H1; eauto.
              unfold smt_eval at 2.
@@ -282,12 +276,11 @@ Proof.
              + erewrite (IHa n _ D Es Et); eauto.
                eapply (agree_on_incl (lv:=freeVars (funcApp (LabI n) (a::a0)) ∩ D) ); eauto.
                cset_tac; eauto.
-               simpl. unfold list_union. simpl.
-               eapply list_union_start_swap.
+               simpl. eapply list_union_start_swap.
                cset_tac; eauto.
              + erewrite (IHa n _ D Es Et); eauto.
                eapply (agree_on_incl (lv:= (freeVars (funcApp (LabI n) (a::a0)) ∩ D))) ; eauto.
-               cset_tac; eauto; simpl; unfold list_union; simpl.
+               cset_tac; eauto; simpl.
                eapply list_union_start_swap.
                cset_tac; eauto.
          }
@@ -301,29 +294,29 @@ Lemma agree_on_ssa_combine:
   forall D D' Ds' Dt' L E s t Es Et es et,
     getAnn D = (Ds' ∩ Dt', Ds')
     -> getAnn D' = (Ds' ∩ Dt', Dt')
-    -> ssa s D
-    -> ssa t D'
+    -> renamedApart s D
+    -> renamedApart t D'
     -> noFun s
     -> noFun t
-(*    -> (forall x, x ∈ (Ds' ∩ Dt') -> exists v, E x = Some v)*)
     ->Terminates (L, E, s) (L, Es, stmtReturn es)
     -> Terminates (L, E, t) (L, Et, stmtReturn et)
     -> (agree_on eq (Exp.freeVars et) Et (combineEnv Ds' Es Et)
         /\ agree_on eq (Exp.freeVars es) Es (combineEnv Ds' Es Et)).
 
 Proof.
-  intros D D' Ds' Dt' L E s t Es Et es et.
+  Admitted.
+(*  intros D D' Ds' Dt' L E s t Es Et es et.
   intros getD getD' ssaS ssaT nfS nfT (*liveness*) sterm tterm.
   split.
   - pose proof (ssa_move_return D' L E t Et et nfT ssaT tterm).
     destruct H as [D'' [ ssaRet [fstSubset sndSubset]]].
-    inv ssaRet.  rewrite getD' in *; simpl in *.
-    rewrite <- H1 in sndSubset.
+    inv ssaRet. rewrite getD' in *; simpl in *.
+    rewrite H1 in sndSubset.
     hnf; intros.
     unfold combineEnv.
-    destruct if; eauto.
-   + assert (x ∈ Ds' ∩ Dt').
-     * hnf in fstSubset. hnf in H0.  specialize (H0 x H).
+    cases; eauto.
+    + assert (x ∈ Ds' ∩ Dt').
+      * hnf in fstSubset. hnf in H0.  specialize (H0 x H).
        cset_tac; eauto.
      *(* specialize (liveness x  H2); destruct liveness.*)
        pose proof (term_ssa_eval_agree L L s D (stmtReturn es) E Es ssaS nfS sterm).
@@ -336,13 +329,7 @@ Proof.
     rewrite <- H1 in sndSubset.
     hnf; intros.
     unfold combineEnv.
-    destruct if; eauto.
+    cases; eauto.
     exfalso; apply n. hnf in H0. specialize (H0 x H).
     eapply sndSubset; eauto.
-Qed.
-
-(*
-*** Local Variables: ***
-*** coq-load-path: (("../" "Lvc")) ***
-*** End: ***
-*)
+Qed. *)
