TransVal/ComputeProps.v
@@ -1,9 +1,10 @@
 Require Import List Arith.
-Require Import IL Annotation AutoIndTac Bisim Exp MoreExp Coherence Fresh Util.
-Require Import SetOperations Sim Var.
-Require Import bitvec smt nofun noGoto freeVars.
+Require Import AutoIndTac Annotation Exp IL MoreExp RenamedApart Util.
+Require Import SetOperations Sim.
+Require Import bitvec smt nofun freeVars.
 Require Import Compute Guards ILFtoSMT tvalTactics TUtil GuardProps.
 
+(*
 (** TODO Remove as unused **)
 Lemma exp_eval_if_list_eval:
   forall el E vl,
@@ -21,7 +22,7 @@ general induction el.
      * exfalso. apply n. rewrite H; reflexivity.
      * destruct (IHel H).  exists x1.
        rewrite H0. reflexivity.
-Qed.
+Qed. *)
 
 (** Lemma 2 in Thesis
 Proves that Terminates ignores the label environment **)
@@ -51,8 +52,8 @@ intros term. general induction term.
   instantiate(1:=EvtTau); subst.
     * econstructor; eauto.
     * intros; isabsurd.
-  + subst; isabsurd.
-  +  pose( L2' := {| F.block_E := E'; F.block_Z := Z; F.block_s := s |} :: L2).
+  + subst. specialize (H0 l Y); isabsurd.
+  +  pose( L2' := F.mkBlocks E s ++ L2).
      specialize (IHterm L' L2' L1' E' V' s' s'0).
      destruct IHterm; eauto; subst.
      exists x. econstructor; eauto.
@@ -68,26 +69,26 @@ Qed.
 
 (** Part 1 of Lemma 1 in the Thesis **)
 Lemma term_ssa_eval_agree L L' s D s' (E:onv val) (E':onv val)
- : ssa s D
+ : renamedApart s D
    -> noFun s
    -> Terminates (L, E, s) (L', E', s')
-   -> agree_on eq (fst (getAnn D)) E E'.
+   -> agree_on eq (fst(getAnn D)) E E'.
 
 Proof.
   intros.
-  general induction H1; invt ssa; try invt F.step;try invt noFun; simpl;
-  try reflexivity; isabsurd.
+  general induction H1; invt renamedApart; try invt F.step;try invt noFun; simpl;
+  try reflexivity.
   - exploit IHTerminates; [ | | reflexivity | reflexivity |]; eauto.
-   rewrite H7 in X; simpl in *. cset_tac; intuition.
-   hnf. hnf in X. intros.
-   unfold update in X. specialize (X x0).
-   assert (x0 ∈ D0 ++ {x; {}}) by (cset_tac; left; assumption).
-   specialize (X H10). decide (x === x0); eauto.
-    + rewrite  <- e0 in H8; exfalso; apply H4 ; assumption.
+    rewrite H8 in H9; simpl in *. cset_tac.
+    hnf in *. intros x0 inD0.
+    specialize (H9 x0).
+    assert (x0 ∈ {x; D0}) by (cset_tac; left; assumption).
+   specialize (H9 H11). unfold update in H9. cases in H9; eauto.
   - exploit IHTerminates; [ | | reflexivity | reflexivity |]; eauto.
-    rewrite H9 in X; simpl in *. assumption.
+    rewrite H9 in H11; simpl in *. assumption.
   - exploit IHTerminates; [| | reflexivity | reflexivity |]; eauto.
-    rewrite H10 in X; simpl in *; assumption.
+    rewrite H10 in H11; simpl in *; assumption.
+  - specialize (H0 f Y); isabsurd.
 Qed.
 
 Lemma terminates_impl_star2:
@@ -95,26 +96,27 @@ Lemma terminates_impl_star2:
     noFun s
     -> Terminates (L, E ,s ) (L', Es, s')
     -> (star2 F.step (L, E, s) nil (L', Es, s'))
-       /\ ((exists e, s' = stmtReturn e) \/ (exists f X, s' = stmtGoto f X)).
+       /\ ((exists e, s' = stmtReturn e) \/ (exists f X, s' = stmtApp f X)).
 
 Proof.
-intros.
-general induction H0; eauto.
--split; eauto; econstructor.
-- split; eauto; econstructor.
-- inversion H2; subst; try isabsurd.
-  + exploit (IHTerminates L' E' s'); try reflexivity.
+  intros L E s L' Es s' noFun_s Terminates_s.
+  general induction Terminates_s.
+  - split; eauto; econstructor.
+  - split; eauto; econstructor.
+  - inversion noFun_s; subst; try isabsurd.
+    + exploit (IHTerminates_s L' E' s'); try reflexivity.
+      * inversion H; subst; eauto.
+      * destruct H2 as [step H2]; split.
+        { change (star2 F.step (L0, E0, stmtLet x e s) (filter_tau EvtTau nil) (L'0, Es, s'0)).
+          econstructor; eauto. destruct a; eauto; isabsurd. }
+        { destruct H2; eauto. }
+  + exploit (IHTerminates_s L' E' s'); eauto.
     * inversion H; subst; eauto.
-    * destruct X as [step X]; split.
-      { change (star2 F.step (L0, E0, stmtExp x e s) (filter_tau EvtTau nil) (L'0, Es, s'0)).
-        econstructor; eauto. destruct a; eauto; isabsurd. }
-      { destruct X; eauto. }
-  + exploit (IHTerminates L' E' s'); eauto.
-    * inversion H; subst; eauto.
-    * destruct X as [step X]; split.
+    * destruct H3 as [step H3]; split.
       { change (star2 F.step (L0, E0, stmtIf e s t)(filter_tau EvtTau nil) (L'0, Es, s'0)).
         econstructor; eauto; destruct a; eauto; isabsurd. }
-      {destruct X; eauto. }
+      {destruct H3; eauto. }
+  + specialize (H0 l Y); isabsurd.
 Qed.
 
 (** Lemma 13 in Thesis
@@ -122,26 +124,26 @@ Proves that all terminating source translations can be modeled
 with the end environment **)
 Lemma terminates_impl_models :
 forall L s D E s' E',
-ssa  s D
+renamedApart s D
 -> noFun s
 -> Terminates (L,E, s) (L, E', s')
 ->  models (fun (f:pred) (x:vallst) => true)  (to_total E')  (translateStmt s source).
 
 Proof.
-intros.
-general induction H1; simpl.
+intros L s D E s' E' ren_s noFun_s Term_s.
+general induction Term_s; simpl.
 - assert (X: models (fun (_:pred) (_:vallst) => true) (to_total E0) (funcApp (LabI 0) (e::nil))).
   + simpl; intuition.
   + eapply models_guardGen_source; simpl. split; eauto.
       eapply (guard_true_if_eval); eauto.
 - eapply models_guardGen_source; simpl; split; eauto.
   eapply (guardList_true_if_eval _ E0); eauto.
-- inv H; invt ssa; invt noFun; simpl in * |- *; subst.
+- inv H; invt renamedApart; invt noFun; simpl in * |- *; subst.
   + eapply models_guardGen_source; simpl; split; eauto.
     * eapply (guard_true_if_eval _ E'0 e v ); eauto.
       eapply exp_eval_agree; eauto.
       assert (A: agree_on eq (fst (getAnn (ann1 (D0, D') an))) E0 E'0).
-      { eapply (term_ssa_eval_agree L' L' (stmtExp x e s') _ s'0 _ _);
+      { eapply (term_ssa_eval_agree L' L' (stmtLet x e s') _ s'0 _ _);
         econstructor; eauto. }
       { eapply (agree_on_incl  (bv:=Exp.freeVars e) (lv:=fst (getAnn (ann1 (D0, D') an)))); eauto. }
     * split; eauto; subst.
@@ -149,12 +151,12 @@ general induction H1; simpl.
       { eapply (exp_eval_agree (E:= E0[x <- Some v])) ; eauto.
         - simpl. eapply (agree_on_incl (bv:={x} ) (lv:= fst (getAnn an))); subst.
           + eapply (term_ssa_eval_agree L' L' s' _ s'0 _ E'0); eauto.
-          + rewrite H11. unfold fst. cset_tac. right; rewrite H4; reflexivity.
+          + rewrite H9. unfold fst. cset_tac.
         - unfold exp_eval. unfold update. decide (x===x); eauto; isabsurd. }
       assert (X2: exp_eval E'0 e = Some v).
       { eapply exp_eval_agree; eauto.
       assert (A: agree_on eq (fst (getAnn (ann1 (D0, D') an))) E0 E'0).
-        - eapply (term_ssa_eval_agree L' L' (stmtExp x e s') _ s'0 _ _);
+        - eapply (term_ssa_eval_agree L' L' (stmtLet x e s') _ s'0 _ _);
           econstructor; eauto.
         - eapply (agree_on_incl  (bv:=Exp.freeVars e) (lv:=fst (getAnn (ann1 (D0, D') an)))); eauto. }
       {  unfold smt_eval;
@@ -162,24 +164,22 @@ general induction H1; simpl.
          eapply  bvEq_equiv_eq; reflexivity. }
   + assert (X: models  (fun (_:pred) (_:vallst) => true) (to_total E'0) ( ite e (translateStmt s' source) (translateStmt b2 source))).
     * simpl.
-      assert (Exp.freeVars e ⊆ fst (getAnn (ann2 (D0, D') ans ant)))
-        by (hnf; intros; hnf in H7; specialize (H7 a); exact (H7 H4)).
+      assert (Exp.freeVars e ⊆ fst (getAnn (ann2 (D0, D') ans ant))) by cset_tac.
       assert (agree_on eq (fst (getAnn (ann2 (D0, D') ans ant))) E' E'0)
         by ( eapply (term_ssa_eval_agree L' L' (stmtIf e s' b2) _ s'0 _ _); econstructor; eauto).
       unfold smt_eval.
-      erewrite (exp_eval_agree (E:=to_partial (to_total E')) (E':=to_partial (to_total E'0))); eauto. simpl.
-      erewrite exp_eval_partial_total; eauto.
-      rewrite condTrue.
-      eapply IHTerminates; eauto.
-      eapply (agree_on_incl (bv:= Exp.freeVars e) (lv:= fst (getAnn (ann2 (D0, D') ans ant)))); eauto.
-      simpl.
-      eapply agree_on_partial; eauto.
-      eapply agree_on_total; eauto.
+      erewrite (exp_eval_agree (E:=to_partial (to_total E')) (E':=to_partial (to_total E'0))); eauto.
+      { erewrite exp_eval_partial_total; eauto.
+        rewrite condTrue.
+        eapply IHTerm_s; eauto. }
+      { eapply (agree_on_incl (bv:= Exp.freeVars e) (lv:= fst (getAnn (ann2 (D0, D') ans ant)))); eauto.
+        simpl.
+        eapply agree_on_partial; eauto.
+        eapply agree_on_total; eauto. }
     * erewrite models_guardGen_source.
       simpl.
       pose proof (guard_true_if_eval  (fun (_:pred) (_:vallst) => true) E'0 e v); eauto.
-      assert (Exp.freeVars e ⊆ fst (getAnn (ann2 (D0, D') ans ant)))
-        by (hnf; intros; hnf in H7; specialize (H7 a); hnf; cset_tac; simpl;  exact (H7 H5)).
+      assert (Exp.freeVars e ⊆ fst (getAnn (ann2 (D0, D') ans ant))) by cset_tac.
       assert (agree_on eq (fst (getAnn (ann2 (D0, D') ans ant))) E' E'0)
         by ( eapply (term_ssa_eval_agree L' L' (stmtIf e s' b2) _ s'0 _ _); econstructor; eauto).
       assert (exp_eval E'0 e = Some v)
@@ -188,23 +188,20 @@ general induction H1; simpl.
       split; eauto.
   + assert (X: models  (fun (_:pred) (_:vallst) => true) (to_total E'0) ( ite e (translateStmt b1 source) (translateStmt s' source))).
     * simpl.
-      assert (Exp.freeVars e ⊆ fst (getAnn (ann2 (D0, D') ans ant)))
-        by (hnf; intros; hnf in H7; specialize (H7 a); exact (H7 H4)).
+      assert (Exp.freeVars e ⊆ fst (getAnn (ann2 (D0, D') ans ant))) by cset_tac.
       assert (agree_on eq (fst (getAnn (ann2 (D0, D') ans ant))) E' E'0)
       by ( eapply (term_ssa_eval_agree L' L' (stmtIf e b1 s') _ s'0 _ _);econstructor;  eauto).
       unfold smt_eval.
       erewrite (exp_eval_agree (E:=to_partial (to_total E')) (E':=to_partial (to_total E'0))); eauto. simpl.
       erewrite exp_eval_partial_total; eauto.
       rewrite condFalse.
-      eapply IHTerminates; eauto.
+      eapply IHTerm_s; eauto.
       eapply (agree_on_incl (bv:= Exp.freeVars e) (lv:= fst (getAnn (ann2 (D0, D') ans ant)))); eauto.
       eapply agree_on_partial, agree_on_total; eauto.
     * erewrite models_guardGen_source; simpl.
       simpl; split; eauto.
       eapply (guard_true_if_eval  (fun (_:pred) (_:vallst) => true) E'0 e v); eauto.
-      assert (Exp.freeVars e ⊆ fst (getAnn (ann2 (D0, D') ans ant)))
-        by (hnf; intros; hnf in H7; specialize (H7 a); hnf; cset_tac;
-            simpl;  exact (H7 H4)).
+      assert (Exp.freeVars e ⊆ fst (getAnn (ann2 (D0, D') ans ant))) by cset_tac.
       assert (agree_on eq (fst (getAnn (ann2 (D0, D') ans ant))) E' E'0)
         by ( eapply (term_ssa_eval_agree L' L' (stmtIf e b1 s') _ s'0 _ _);
              econstructor; eauto).
@@ -226,13 +223,14 @@ intros. general induction H0.
   + inversion H2; subst; try isabsurd.
     * inversion H. rewrite <- H13; eauto.
     * inversion H;  rewrite <- H14; eauto.
-  + inversion H; subst; eauto; isabsurd.
+    * specialize (H1 l Y); isabsurd.
+  + inversion H; subst; eauto; isabsurd. specialize (H1 l Y); isabsurd.
 Qed.
 
 Lemma terminates_impl_evalList:
 forall L  L' E s E' f el,
 noFun s
--> Terminates (L, E, s) (L', E', stmtGoto f el)
+-> Terminates (L, E, s) (L', E', stmtApp f el)
 -> exists v, omap (exp_eval E') el = Some v.
 
 Proof.
@@ -240,7 +238,9 @@ intros. general induction H0.
 - exists vl; eauto.
 - exploit (IHTerminates L0 L'0 E' s' E'0 f el); eauto.
   + inversion H2; subst; inversion H; subst; eauto; isabsurd.
+    specialize (H1 l Y); isabsurd.
   + inversion H; subst; eauto; isabsurd.
+    specialize (H1 l Y); isabsurd.
 Qed.
 
 (** Lemma cannot be proven with star2 step because in the
@@ -248,30 +248,32 @@ goto case, ssa is not proven! **)
 Lemma ssa_move_return:
   forall D (L:F.labenv) E s E' e,
     noFun s
-    -> ssa s D
+    -> renamedApart s D
     -> Terminates (L, E, s) (L, E', stmtReturn e)
-    -> exists D', ssa (stmtReturn e) D'
+    -> exists D', renamedApart (stmtReturn e) D'
                   /\ fst (getAnn D) ⊆ fst (getAnn D')
                   /\ snd (getAnn D') ⊆ snd (getAnn D).
 
 Proof.
   intros. general induction H1.
-  - exists D. split; eauto. split; cset_tac; eauto.
- -  inversion H3; subst; isabsurd.
+  - exists D. split; eauto.
+  - inversion H3; subst; isabsurd.
     + inversion H; inversion H2; subst. exploit (IHTerminates an L' (E0[x<-Some v]) s' ); eauto.
-      destruct X. exists x0.
-      destruct H8 as [H8 [H9 H10]].
-      split; eauto; split;  simpl; cset_tac; rewrite H7 in *;
-      simpl in *; hnf in *; eauto. eapply H9; cset_tac; eauto.
+      destruct H9. exists x0.
+      destruct H9 as [H9 [H10 H11]].
+      split; eauto; split;  simpl; cset_tac; rewrite H8 in *;
+        simpl in *; hnf in *; eauto.
+      * eapply H10; cset_tac; eauto.
+      * apply H7. right; apply H11; eauto.
     + inversion H; inversion H2; subst.
       * exploit (IHTerminates ans); eauto.
-        destruct X. exists x.
+        destruct H11. exists x.
         destruct H11 as [ H11 [ H12 H13]].
         split; eauto; split; simpl; cset_tac; rewrite H9 in *;
         simpl in *; hnf in *; eauto. eapply H6.
         left; eapply H13; eauto.
       * exploit (IHTerminates ant); eauto.
-        destruct X; exists x.
+        destruct H11; exists x.
         destruct H11 as [ H11 [ H12 H13]].
         split; eauto; split; simpl; cset_tac; rewrite H10 in *;
         simpl in *; hnf in *; eauto; eapply H6.
@@ -282,33 +284,34 @@ Qed.
 Lemma ssa_move_goto:
   forall D (L:F.labenv) E s E' f el,
     noFun s
-    -> ssa s D
-    -> Terminates (L, E, s) (L, E', stmtGoto f el)
-    -> exists D', ssa (stmtGoto f el) D'
+    -> renamedApart s D
+    -> Terminates (L, E, s) (L, E', stmtApp f el)
+    -> exists D', renamedApart (stmtApp f el) D'
                   /\ fst (getAnn D) ⊆ fst (getAnn D')
                   /\ snd (getAnn D') ⊆ snd (getAnn D).
 
 Proof.
   intros D L E s E' f el nfS ssaS sterm.
   general induction sterm.
-  - exists D; eauto. split; eauto; split; cset_tac; eauto.
+  - exists D; eauto.
   - inversion ssaS; subst; try isabsurd.
     + inversion nfS; inversion ssaS; inversion H;
       subst; exploit (IHsterm an L' (E0 [ x<- Some v]) s'); eauto.
-      destruct X as [D'' [ssaGoto [fstSubset sndSubset]]].
+      destruct H6 as [D'' [ssaGoto [fstSubset sndSubset]]].
       exists D''; simpl.
-      split; eauto; split; cset_tac; rewrite H18 in *;
-      simpl in *; hnf in *; eauto.
-      eapply fstSubset. cset_tac; eauto.
-    +  inversion nfS; inversion ssaS; inversion H; subst.
+      split; eauto; split; cset_tac.
+      * apply fstSubset. rewrite H5; simpl. cset_tac.
+      * apply H19. rewrite H20 in sndSubset; simpl in *. right.
+        cset_tac.
+    + inversion nfS; inversion ssaS; inversion H; subst.
        * exploit (IHsterm ans); eauto.
-         destruct X as [D'' [ssaGoto [fstSubset sndSubset]]].
+         destruct H8 as [D'' [ssaGoto [fstSubset sndSubset]]].
          exists D''; simpl.
          split; eauto. split; simpl; cset_tac; rewrite H25 in *;
          simpl in *; hnf in *; eauto.
          eapply H22. left; eapply sndSubset; eauto.
        * exploit (IHsterm ant); eauto.
-         destruct X as [D'' [ssaGoto [fstSubset sndSubset]]].
+         destruct H8 as [D'' [ssaGoto [fstSubset sndSubset]]].
          exists D''; simpl.
          split; eauto.
          split; cset_tac; rewrite H26 in *; simpl in *;
@@ -338,64 +341,60 @@ Proof.
     + exists EvtTau. exists ( L1, V[x1 <- Some v], b). econstructor; eauto.
     + exists EvtTau; exists (L1, V, b1); econstructor; eauto.
     + exists EvtTau; exists (L1, V, b2); econstructor; eauto.
+    + subst. specialize (H l Y); isabsurd.
     + exists EvtTau.
-        exists ({| F.block_E := V; F.block_Z := Z; F.block_s := s |}::L1, V, t).
+      exists (F.mkBlocks V s ++ L1, V, t).
         econstructor; eauto.
     + exists x; subst.
         exists (L1, V[x1 <- Some v], s).
         econstructor; eauto.
-   - inversion H.
+   - inversion H; subst.
      + specialize (IHcrash L1 L2 L1' (V[x<-Some v]) V' b s').
        destruct IHcrash; eauto.
        eexists; econstructor; eauto.
        * instantiate (1:= EvtTau); econstructor; eauto.
-       * intros; isabsurd.
      + specialize (IHcrash L1 L2 L1' V V' b1 s').
        destruct IHcrash; eauto.
        eexists; econstructor; eauto.
        * instantiate (1:=EvtTau); econstructor; eauto.
-       * intros; isabsurd.
      + specialize (IHcrash L1 L2 L1' V V' b2 s').
        destruct IHcrash; eauto.
        eexists; econstructor; eauto.
        * instantiate (1:=EvtTau); econstructor; eauto.
-       * intros; isabsurd.
-     + isabsurd.
-     + pose (L2' := {| F.block_E := V; F.block_Z := Z; F.block_s := s |}::L2).
-       specialize (IHcrash ({| F.block_E := V; F.block_Z := Z; F.block_s := s |}::L1) L2' L1' V V' t s').
+     + specialize (H0 l Y); isabsurd.
+     + pose (L2' := F.mkBlocks V s ++ L2).
+       specialize (IHcrash (F.mkBlocks V s ++ L1) L2' L1' V V' t s').
        destruct IHcrash; eauto.
        eexists; econstructor; eauto.
        * instantiate (1:= EvtTau); econstructor; eauto.
-       * intros; isabsurd.
      + specialize (IHcrash  L1 L2 L1' (V[x<-Some v]) V' s s').
        destruct IHcrash; eauto.
        eexists; econstructor; eauto.
-       * instantiate (1:=a); subst; econstructor; eauto.
-       * intros; isabsurd.
+       * instantiate (1:=EvtExtern {| extern_fnc := f; extern_args := vl; extern_res := v |}); subst; econstructor; eauto.
 Qed.
 
 (** Part 2 of Lemma 1 in the Thesis *)
 Lemma crash_ssa_eval_agree L L' s D s' (E:onv val) (E':onv val)
-: ssa s D
+: renamedApart s D
   ->noFun s
   -> Crash (L, E, s) (L', E', s')
   -> agree_on eq (fst (getAnn (D))) E E'.
 
 Proof.
   intros.
-  general induction H1; invt ssa; try invt F.step; try invt noFun; simpl;
-  try reflexivity; isabsurd.
+  general induction H1; invt renamedApart; try invt F.step; try invt noFun; simpl;
+  try reflexivity.
   - exploit IHCrash; [ | | reflexivity | reflexivity |]; eauto.
-    rewrite H7 in X; simpl in *; cset_tac; intuition.
-    hnf; hnf in X; intros.
-    unfold update in X; specialize (X x0).
-    assert (x0 ∈ D0 ++ {x; {}}) by (cset_tac; left; assumption).
-    specialize (X H10); decide (x === x0); eauto.
-    + rewrite <- e0 in H8; exfalso; eapply H4; assumption.
+    rewrite H8 in H9; unfold update in H9.
+    simpl in *. hnf; hnf in H9; intros x0 inD0.
+    specialize (H9 x0).
+    assert (x0 ∈ {x; D0}) by cset_tac.
+    specialize (H9 H11); cases in H9; eauto.
   - exploit IHCrash; [ | | reflexivity | reflexivity |]; eauto.
-    rewrite H9 in X; eauto.
+    rewrite H9 in H11; eauto.
   - exploit IHCrash; [ | | reflexivity | reflexivity |]; eauto.
-    rewrite H10 in X; eauto.
+    rewrite H10 in H11; eauto.
+  - specialize (H0 f Y); isabsurd.
 Qed.
 
 Lemma crash_impl_err:
@@ -416,21 +415,22 @@ Proof.
 - destruct sigma'. destruct p. inversion nf; subst; try isabsurd.
   + exploit (IHCrash o s1 Es s' l L') ; try reflexivity; eauto; subst.
     * inversion H; eauto.
-    * destruct X; split; eauto.
-      change (star2 F.step (L0, E0, stmtExp x e s1) (filter_tau EvtTau nil) (L', Es, s')).
+    * destruct H2; split; eauto.
+      change (star2 F.step (L0, E0, stmtLet x e s1) (filter_tau EvtTau nil) (L', Es, s')).
       econstructor; eauto. destruct a; eauto; isabsurd.
   + inversion H; exploit (IHCrash o s Es s' l L'); subst; eauto.
-    * destruct X; split; eauto.
+    * split; eauto.
       change (star2 F.step (l, o, stmtIf e s t) (filter_tau EvtTau nil) (L', Es, s')).
       econstructor; eauto.
-    * destruct X; split; eauto.
+    * split; eauto.
       change (star2 F.step (l, o, stmtIf e s1 s) (filter_tau EvtTau nil) (L', Es, s')).
       econstructor; eauto.
+  + specialize (H0 l0 Y); isabsurd.
 Qed.
 
 Lemma nostep_let:
 forall L E x e s,
-normal2 F.step (L, E, stmtExp x e s)
+normal2 F.step (L, E, stmtLet x e s)
 -> exp_eval E e = None.
 
 Proof.
@@ -458,7 +458,7 @@ Proves that crashing target programs can be modeled by any
 predicate environment and the environment in which they crash **)
 Lemma crash_impl_models:
   forall L L' D s E Es s',
-    ssa s D
+    renamedApart s D
     -> (forall x, x ∈ fst(getAnn D) -> exists v, E x = Some v)
     -> noFun s
     -> Crash (L, E, s) (L', Es, s')
@@ -480,7 +480,7 @@ Proof.
     +pose proof (nostep_let L0 E0 x e s H0).
         pose proof (undef_models F  E0 e).
         assert (forall x, x ∈ Exp.freeVars e -> exists v, E0 x = Some v).
-     * intros; invt ssa. specialize (H3 x0). eapply H3.
+     * intros; invt renamedApart. specialize (H3 x0). eapply H3.
        simpl; cset_tac; eauto.
       (** Contradiction: The expression does not evaluate, but the guard
        is satisfiable --> undef_models as contradiction **)
@@ -489,36 +489,35 @@ Proof.
     + pose proof (nostep_if L0 E0 e s t H0).
       pose proof (undef_models F  E0 e).
      assert (forall x, x ∈ Exp.freeVars e -> exists v, E0 x = Some v).
-     * intros; invt ssa. eapply (H3 x). simpl; cset_tac; eauto.
+     * intros; invt renamedApart. eapply (H3 x). simpl; cset_tac; eauto.
        (** Same contradiction **)
      * specialize (H9 H10 H8 H7); isabsurd.
     + pose proof (undef_models F E0 e).
          assert (forall x, x ∈ Exp.freeVars e -> exists v, E0 x = Some v).
-        { intros; inversion H2; cset_tac.  simpl in H3. specialize (H3 x).
-        destruct H1; eauto. }
-       { eapply H7; eauto. }
+        { intros; inversion H2; cset_tac. }
+        { eapply H7; eauto. }
        (** C-Step **)
   - destruct sigma' as  [[L E'] sc].
     inversion H; intros; subst; try isabsurd;
-    invt ssa; invt noFun; subst; simpl;
+    invt renamedApart; invt noFun; subst; simpl;
     eapply models_guardGen_target; simpl; intros.
     + split.
      Focus 2.
      exploit (IHCrash L L' an sc (E0 [x<-Some v]) Es s'); eauto; intros.
-     unfold update. destruct if; eauto.
+     unfold update. cases; eauto.
      destruct (H3 x0); eauto; simpl.
-     rewrite H12 in H7; simpl in H7. cset_tac. destruct H7; eauto; isabsurd.
+     rewrite H13 in H7; simpl in H7. cset_tac.
     * assert ( exp_eval Es e = Some v /\ exp_eval Es (Var x) = Some v).
     { split.
       - eapply (exp_eval_agree (E:=E0)); eauto.
         hnf. intros.  hnf in H9. specialize (H9 x0 H7).
-        pose proof (crash_ssa_eval_agree L L' (stmtExp x e sc) (ann1 (D0, D') an) s' E0 Es).
-        eapply H10; eauto; econstructor; eauto.
+        eapply (crash_ssa_eval_agree L L' (stmtLet x e sc) (ann1 (D0, D') an) s' E0 Es);
+          eauto; econstructor; eauto.
       - eapply (exp_eval_agree (E:= E0[x<-Some v])).
         + hnf. intros; simpl in *.
           eapply (crash_ssa_eval_agree L L' sc an s' (E0[x<-Some v]) Es); eauto.
-          rewrite H12; simpl. cset_tac. right. rewrite H7; eauto.
-        + simpl. unfold update. decide (x === x); eauto; isabsurd.
+          rewrite H13; simpl. cset_tac.
+        + simpl. unfold update. cases; eauto; isabsurd.
           }
     { destruct H7.
       unfold smt_eval.
@@ -544,10 +543,5 @@ Proof.
          rewrite condFalse.
          eapply (IHCrash L L' ant sc E' Es s'); eauto.
          intros. rewrite H15 in H13. simpl in *; eauto.
+    + apply (H0 l Y); auto.
 Qed.
-
-(*
-*** Local Variables: ***
-*** coq-load-path: (("../" "Lvc")) ***
-*** End: ***
-*)
